Std/Data/HashMap/Lemmas.lean
@@ -4,12 +4,59 @@ Released under Apache 2.0 license as described in the file LICENSE.
 Authors: Scott Morrison
 -/
 import Std.Data.HashMap.Basic
+import Std.Data.HashMap.WF
 import Std.Util.ProofWanted
 
 namespace Std.HashMap
 
-@[simp] proof_wanted empty_find? [BEq α] [Hashable α] {a : α} :
-    (∅ : HashMap α β).find? a = none
+/--
+Any hash map of size zero has no accessible elements.
+-/
+theorem find?_none_of_size_zero [BEq α] [Hashable α] (m : HashMap α β) :
+    m.size = 0 → ∀ (a : α), m.find? a = none := by
+  simp[HashMap.size,(Imp.WF.out m.property).left,Imp.Buckets.size,Nat.sum_eq_zero_iff]
+  intro h k
+  simp[HashMap.find?,HashMap.Imp.find?]
+  suffices AssocList.toList _ = [] by rw[this] ; simp
+  exact List.length_eq_zero.mp (h _ (by rw[Array.getElem_eq_data_get] ; apply List.get_mem))
 
-proof_wanted insert_find? [BEq α] [Hashable α] (m : HashMap α β) (a a' : α) (b : β) :
-    (m.insert a b).find? a' = if a' == a then some b else m.find? a'
+/--
+A hash map with no accessible elements is size zero under the assumption that every key `a` in `α`
+is accessible by some key `b` in `α`, where `a == b` and `hash a = hash b`.
+This condition is trivially satisfied when `==` over `α` is reflexive.
+-/
+theorem size_zero_of_find?_none [BEq α] [Hashable α] (m : HashMap α β)
+    (accessibility : ∀ a : α, ∃ b : α, a == b ∧ hash a = hash b) :
+    (∀ (a : α), m.find? a = none) → m.size = 0 := by
+  simp[HashMap.size,Imp.WF.out m.property,Imp.Buckets.size,Nat.sum_eq_zero_iff]
+  intro h a h₀
+  cases a with
+  | nil => simp
+  | cons k v a' =>
+    have ⟨k',hk'⟩ := accessibility k
+    suffices m.find? k' = some v by simp[h] at this
+    simp[List.mem_iff_get] at h₀
+    let ⟨i,h₀⟩ := h₀
+    have := (Imp.WF.out m.property).right.hash_self i i.isLt
+    simp[Array.getElem_eq_data_get] at this
+    rw[h₀] at this
+    simp[AssocList.All] at this
+    simp[HashMap.find?,HashMap.Imp.find?,Imp.mkIdx,this.left,Array.getElem_eq_data_get,←hk'.right]
+    rw[h₀]
+    simp[List.find?,hk'.left]
+
+/--
+The empty hash map `∅` has no accessible elements.
+-/
+@[simp] theorem empty_find? [BEq α] [Hashable α] {a : α} :
+    (∅ : HashMap α β).find? a = none := by
+  apply find?_none_of_size_zero ; rfl
+
+/--
+Insertion behaves correctly with respect to the `find?` operation when the hash is lawful and
+boolean equality is sane.
+-/
+theorem insert_find? [BEq α] [Hashable α] [PartialEquivBEq α] [LawfulHashable α]
+    (m : HashMap α β) (a a' : α) (b : β) :
+    (m.insert a b).find? a' = if a' == a then some b else m.find? a' := by
+  exact Imp.insert_find? (Imp.WF.out m.property).2
